progs/verif_sumarray.v
@@ -156,7 +156,8 @@ apply (remember_value (eval_var _four (tarray tint 4))); intro a0.
 forward.  (*  r = sumarray(four,4); *)
 instantiate (1:= (a0,Ews,four_contents,4)) in (Value of witness).
  entailer!. 
-   intros. unfold four_contents. apply ZnthV_map_Vint_is_int. apply H2.
+   intros. unfold four_contents. apply ZnthV_map_Vint_is_int.
+ split; auto.
  auto with closed.
  forward. (* return s; *)
  unfold main_post. entailer!.
