sha/verif_sha_update3.v
@@ -123,7 +123,7 @@ rewrite array_at_tuchar_isbyteZ.
  rewrite (prop_true_andp (Forall _ data)) by auto.
  rewrite negb_false_iff in H5.
  apply ltu_repr in H5; [ | repable_signed | omega].
- clear TC1 TC.
+ clear TC.
  fold t_struct_SHA256state_st.
  unfold k in H0,H5.
  rewrite (prop_true_andp (_ /\ _)).
